general update on latest work, add a file (robust-imp-comments.org) with comments about coq development

RSC_DC_MD.v
@@ -10,6 +10,7 @@ Require Import Source.PS.
 Require Import Intermediate.Machine.
 Require Import Intermediate.PS.
 Require Import Intermediate.Decomposition.
+Require Import Intermediate.Composition.
 Require Import S2I.Compiler.
 Require Import S2I.Definitions.
 
@@ -24,7 +25,79 @@ Section RSC_DC_MD.
   Variable p_compiled: Intermediate.program.
   Variable Ct: Intermediate.program.
 
-  Let pCt := Intermediate.program_link p_compiled Ct.
+  Let slink := Source.program_link.
+  Let ilink := Intermediate.program_link.
+
+  (* Some reasonable assumptions about our programs *)
+
+  Hypothesis successfull_compilation:
+    compile_program p = Some p_compiled.
+
+  Hypothesis linkability:
+    Intermediate.linkable_programs p_compiled Ct.
+
+  Hypothesis closedness:
+    Intermediate.closed_program (ilink p_compiled Ct).
+
+  (* some useful functions on closed programs *)
+
+  Definition s_main_comp (p: Source.program): Component.id :=
+    match Source.prog_main p with
+    | Some (mainC, _) => mainC
+    | None => 0
+    end.
+
+  Definition i_main_comp (p: Intermediate.program): Component.id :=
+    match Intermediate.prog_main p with
+    | Some (mainC, _) => mainC
+    | None => 0
+    end.
+
+  (* Some facts (provable and to prove) about linking and compilation *)
+
+  Hypothesis compilation_preserves_interface:
+    forall p p_compiled,
+      (*Source.prog_main p = None -> this is needed because of the main wrapping *)
+      compile_program p = Some p_compiled ->
+      Intermediate.prog_interface p_compiled = Source.prog_interface p.
+
+  (* This should be provable, although we may have to slightly change the compiler *)
+  (* (e.g. procedure id & label generation should be local to the component *)
+  Hypothesis separate_compilation:
+    forall p c p_comp c_comp,
+      Source.linkable_programs p c ->
+      compile_program p = Some p_comp ->
+      compile_program c = Some c_comp ->
+      compile_program (slink p c) = Some (ilink p_comp c_comp).
+
+  Hypothesis compilation_preserves_linkability:
+    forall p p_compiled c c_compiled,
+      Source.linkable_programs p c ->
+      compile_program p = Some p_compiled ->
+      compile_program c = Some c_compiled ->
+      Intermediate.linkable_programs p_compiled c_compiled.
+
+  Hypothesis slink_sym:
+    forall p c,
+      slink p c = slink c p.
+
+  Hypothesis ilink_sym:
+    forall p c,
+      ilink p c = ilink c p.
+
+  (* Definability *)
+
+  Hypothesis definability_with_linking:
+    forall p c t,
+      Intermediate.linkable_programs p c ->
+      Intermediate.closed_program (ilink p c) ->
+      program_behaves (I.CS.sem (ilink p c)) (Terminates t) ->
+    exists p' c',
+      Source.prog_interface p' = Intermediate.prog_interface p /\
+      Source.prog_interface c' = Intermediate.prog_interface c /\
+      Source.linkable_programs p' c' /\
+      Source.closed_program (slink p' c') /\
+      program_behaves (S.CS.sem (slink p' c')) (Terminates t).
 
   (* FCC *)
   Hypothesis I_simulates_S:
@@ -36,6 +109,7 @@ Section RSC_DC_MD.
       forward_simulation (S.CS.sem p) (I.CS.sem tp).
 
   (* BCC *)
+  (* We derive BCC from FCC as in CompCert *)
   Corollary S_simulates_I:
     forall p,
       Source.closed_program p ->
@@ -51,42 +125,111 @@ Section RSC_DC_MD.
     - apply I.CS.determinacy.
   Qed.
 
-  Hypothesis successfull_compilation:
-    compile_program p = Some p_compiled.
-
-  Hypothesis linkability:
-    Intermediate.linkable_programs p_compiled Ct.
-
-  Hypothesis closedness:
-    Intermediate.closed_program pCt.
-
-  Definition main_comp (p: Source.program): Component.id :=
-    match Source.prog_main p with
-    | Some (mainC, _) => mainC
-    | None => 0
-    end.
+  (* Main Theorem *)
 
   Theorem RSC_DC_MD:
     forall t,
-      program_behaves (I.CS.sem pCt) (Terminates t) ->
+      program_behaves (I.CS.sem (ilink p_compiled Ct)) (Terminates t) ->
     exists Cs beh,
       Source.prog_interface Cs = Intermediate.prog_interface Ct /\
       program_behaves (S.CS.sem (Source.program_link p Cs)) beh /\
       exists t',
         (beh = Terminates t' /\ behavior_prefix t (Terminates t')) \/
         (beh = Goes_wrong t' /\ behavior_prefix t' (Terminates t) /\
-         undef_in (main_comp p) t' (Source.prog_interface p)).
+         undef_in (s_main_comp (Source.program_link p Cs)) t' (Source.prog_interface p)).
   Proof.
-    intros t Hbeh. subst pCt.
+    intros t Hbeh.
+
+    (* decomposition *)
     destruct (decomposition_with_refinement linkability Hbeh)
       as [beh' [Hbeh' Hbeh_improves]].
-    inversion Hbeh_improves; subst.
-    - (* apply definability
-         go down with forward simulation (compiler correctness)
-         compose with CC result
-         go up with backward simulation (compiler correctness)
-         reason on who blame when ub *)
+
+    inversion Hbeh_improves; subst;
+      try (destruct H as [? []]; discriminate).
+
+    (* definability *)
+    destruct (definability_with_linking linkability closedness Hbeh)
+      as [P' [Cs [Hsame_iface1 [Hsame_iface2 [P'_Cs_linkability [P'_Cs_closedness HP'_Cs_beh]]]]]].
+
+    (* forward simulation *)
+    assert (exists P'_compiled Cs_compiled,
+               compile_program P' = Some P'_compiled /\
+               compile_program Cs = Some Cs_compiled /\
+               compile_program (slink P' Cs) = Some (ilink P'_compiled Cs_compiled))
+      as HP'_Cs_compiles. {
+      (* the definability output can be splitted in two programs *)
+      (* probably need partialize to obtain them *)
       admit.
-    - destruct H as [? []]. discriminate.
+    }
+    destruct HP'_Cs_compiles
+      as [P'_compiled [Cs_compiled [HP'_compiles [HCs_compiles HP'_Cs_compiles]]]].
+    assert (program_behaves (I.CS.sem (ilink P'_compiled Cs_compiled)) (Terminates t))
+      as HP'_Cs_compiled_beh. {
+      apply forward_simulation_same_safe_behavior
+        with (L2:=I.CS.sem (ilink P'_compiled Cs_compiled)) in HP'_Cs_beh;
+        simpl; eauto.
+      apply I_simulates_S; auto.
+      - apply Source.linking_well_formedness; auto.
+    }
+
+    (* decomposition *)
+    assert (not_wrong (Terminates t)) as Hsafe_beh. { simpl. auto. }
+    pose proof decomposition_with_safe_behavior linkability Hbeh Hsafe_beh as HP_decomp.
+    assert (Intermediate.linkable_programs Cs_compiled P'_compiled) as linkability'. {
+      eapply compilation_preserves_linkability with (p:=Cs) (c:=P'); eauto.
+      apply Source.linkable_sym. auto.
+    }
+    rewrite ilink_sym in HP'_Cs_compiled_beh.
+    pose proof decomposition_with_safe_behavior linkability'
+         HP'_Cs_compiled_beh Hsafe_beh as HCs_decomp.
+
+    (* composition *)
+    assert (Intermediate.prog_interface Ct = Intermediate.prog_interface Cs_compiled)
+      as Hctx_same_iface. {
+      symmetry. erewrite compilation_preserves_interface.
+      rewrite <- Hsame_iface2. reflexivity. auto.
+    }
+    rewrite Hctx_same_iface in HP_decomp.
+    assert (Intermediate.prog_interface p_compiled = Intermediate.prog_interface P'_compiled) as Hprog_same_iface. {
+      symmetry. erewrite compilation_preserves_interface.
+      apply Hsame_iface1. auto.
+    }
+    rewrite <- Hprog_same_iface in HCs_decomp.
+
+    assert (Intermediate.linkable_programs Cs_compiled p_compiled) as linkability''. {
+      admit.
+    }
+    enough (Intermediate.closed_program (ilink Cs_compiled p_compiled))
+      as HpCs_compiled_closed.
+    enough (Intermediate.well_formed_program (ilink Cs_compiled p_compiled))
+      as HpCs_compiled_well_formed.
+    pose proof composition_for_termination linkability'' HpCs_compiled_closed
+         HpCs_compiled_well_formed HCs_decomp HP_decomp as HpCs_compiled_beh.
+
+    (* backward simulation *)
+    assert (exists beh1,
+               program_behaves (S.CS.sem (slink Cs p)) beh1 /\
+               behavior_improves beh1 (Terminates t)) as HpCs_beh. {
+      apply backward_simulation_behavior_improves
+        with (L1:=S.CS.sem (slink Cs p)) in HpCs_compiled_beh; auto.
+      - apply S_simulates_I.
+        + admit.
+        + admit.
+        + admit.
+    }
+    destruct HpCs_beh as [pCs_beh [HpCs_beh HpCs_beh_imp]].
+    exists Cs. exists pCs_beh.
+    repeat split; auto.
+    - erewrite slink_sym. assumption.
+    - inversion HpCs_beh_imp.
+      + exists t. left. split. auto.
+        exists (Terminates E0). simpl. rewrite E0_right. reflexivity.
+      + destruct H as [t' [Hgoes_wrong Hprefix]].
+        exists t'. right. repeat split; auto.
+        (* blame UB *)
+        admit.
+
+    - admit.
+    - admit.
   Admitted.
 End RSC_DC_MD.
