S2I/Examples/DefaultInitBuffer.v
@@ -4,6 +4,6 @@ Require Import S2I.Examples.Helper.
 Require Import Source.Examples.DefaultInitBuffer.
 
 Definition fuel := 1000%nat.
-Definition to_run := compile_and_run default_init_buffer (Int 42) fuel.
+Definition to_run := compile_and_run default_init_buffer fuel.
 
 Extraction "/tmp/run_compiled_default_init_buffer.ml" to_run.
