S2I/Examples/Factorial.v
@@ -4,6 +4,6 @@ Require Import S2I.Examples.Helper.
 Require Import Source.Examples.Factorial.
 
 Definition fuel := 1000.
-Definition to_run := compile_and_run factorial (Int 7) fuel.
+Definition to_run := compile_and_run factorial fuel.
 
 Extraction "/tmp/run_compiled_fact.ml" to_run.
