S2I/Examples/Identity.v
@@ -4,6 +4,6 @@ Require Import S2I.Examples.Helper.
 Require Import Source.Examples.Identity.
 
 Definition fuel := 1000%nat.
-Definition to_run := compile_and_run identity (Int 42) fuel.
+Definition to_run := compile_and_run identity fuel.
 
 Extraction "/tmp/run_compiled_identity.ml" to_run.
