S2I/Examples/Increment.v
@@ -4,6 +4,6 @@ Require Import S2I.Examples.Helper.
 Require Import Source.Examples.Increment.
 
 Definition fuel := 1000%nat.
-Definition to_run := compile_and_run increment (Int 42) fuel.
+Definition to_run := compile_and_run increment fuel.
 
 Extraction "/tmp/run_compiled_increment.ml" to_run.
