S2I/Examples/NestedCalls.v
@@ -4,6 +4,6 @@ Require Import S2I.Examples.Helper.
 Require Import Source.Examples.NestedCalls.
 
 Definition fuel := 1000%nat.
-Definition to_run := compile_and_run nested_calls (Int 1) fuel.
+Definition to_run := compile_and_run nested_calls fuel.
 
 Extraction "/tmp/run_compiled_nested_calls.ml" to_run.
