Source/GlobalEnv.v
@@ -11,15 +11,6 @@ Record global_env : Type := mkGlobalEnv {
   genv_buffers : NMap Block.id
 }.
 
-Record well_formed_global_env (G: global_env) := {
-  wfgenv_interface_soundness:
-    sound_interface (genv_interface G);
-  wfgenv_procedures_soundness:
-    domm (genv_procedures G) = domm (genv_interface G);
-  wfgenv_buffers_soundness:
-    domm (genv_buffers G) = domm (genv_interface G)
-}.
-
 Definition prepare_global_env (p: program) : global_env :=
   {| genv_interface := prog_interface p;
      genv_procedures := prog_procedures p;
